<?xml version="1.0"?>
<rdf:RDF xmlns="http://purl.org/tio/ns#"
     xml:base="http://purl.org/tio/ns"
     xmlns:dc="http://purl.org/dc/elements/1.1/"
     xmlns:gr="http://purl.org/goodrelations/v1#"
     xmlns:owl="http://www.w3.org/2002/07/owl#"
     xmlns:rdf="http://www.w3.org/1999/02/22-rdf-syntax-ns#"
     xmlns:xml="http://www.w3.org/XML/1998/namespace"
     xmlns:xsd="http://www.w3.org/2001/XMLSchema#"
     xmlns:foaf="http://xmlns.com/foaf/0.1/"
     xmlns:rdfs="http://www.w3.org/2000/01/rdf-schema#"
     xmlns:dcterms="http://purl.org/dc/terms/">
    <owl:Ontology rdf:about="http://purl.org/tio/ns#">
        <owl:imports rdf:resource="http://purl.org/goodrelations/v1"/>
        <dc:contributor xml:lang="en">Some class and property definitions are inspired by or based on abstracts from Wikipedia, the free encyclopedia.</dc:contributor>
        <dc:creator xml:lang="en">Martin Hepp</dc:creator>
        <dc:subject xml:lang="en">E-Commerce, E-Business, GoodRelations, Ontology, Tickets, Transportation, Events, Concerts, Museums</dc:subject>
        <dc:title xml:lang="en">TIO: The TIckets Ontology for Semantic Web-based E-Commerce</dc:title>
        <dcterms:license rdf:resource="http://creativecommons.org/licenses/by/3.0/"/>
        <rdfs:comment xml:lang="en">TIO: The TIckets Ontology
    
A vocabulary for describing tickets for events, transportation, or points of interest for e-commerce.

Vocabulary:    http://purl.org/tio/ns#
Namespace:     http://purl.org/tio/ns#

The Tickets Ontology is designed to be used in combination with GoodRelations, a standard vocabulary for the commercial aspects of offers of tickets.

See http://purl.org/goodrelations/ for more information.</rdfs:comment>
        <rdfs:label xml:lang="en">Tickets Ontology</rdfs:label>
        <rdfs:seeAlso rdf:resource="http://purl.org/goodrelations/"/>
        <owl:versionInfo>V 1.0, Release 2010-11-17</owl:versionInfo>
    </owl:Ontology>
    


    <!-- 
    ///////////////////////////////////////////////////////////////////////////////////////
    //
    // Annotation properties
    //
    ///////////////////////////////////////////////////////////////////////////////////////
     -->

    


    <!-- http://purl.org/dc/elements/1.1/contributor -->

    <owl:AnnotationProperty rdf:about="http://purl.org/dc/elements/1.1/contributor"/>
    


    <!-- http://purl.org/dc/elements/1.1/creator -->

    <owl:AnnotationProperty rdf:about="http://purl.org/dc/elements/1.1/creator"/>
    


    <!-- http://purl.org/dc/elements/1.1/rights -->

    <owl:AnnotationProperty rdf:about="http://purl.org/dc/elements/1.1/rights"/>
    


    <!-- http://purl.org/dc/elements/1.1/subject -->

    <owl:AnnotationProperty rdf:about="http://purl.org/dc/elements/1.1/subject"/>
    


    <!-- http://purl.org/dc/elements/1.1/title -->

    <owl:AnnotationProperty rdf:about="http://purl.org/dc/elements/1.1/title"/>
    


    <!-- http://purl.org/dc/terms/license -->

    <owl:AnnotationProperty rdf:about="http://purl.org/dc/terms/license"/>
    


    <!-- 
    ///////////////////////////////////////////////////////////////////////////////////////
    //
    // Object Properties
    //
    ///////////////////////////////////////////////////////////////////////////////////////
     -->

    


    <!-- http://purl.org/tio/ns#accessTo -->

    <owl:ObjectProperty rdf:about="http://purl.org/tio/ns#accessTo">
        <rdfs:domain>
            <owl:Class>
                <owl:unionOf rdf:parseType="Collection">
                    <rdf:Description rdf:about="http://purl.org/tio/ns#ScopeOfAccess"/>
                    <rdf:Description rdf:about="http://purl.org/tio/ns#Ticket"/>
                </owl:unionOf>
            </owl:Class>
        </rdfs:domain>
        <rdfs:range>
            <owl:Class>
                <owl:unionOf rdf:parseType="Collection">
                    <rdf:Description rdf:about="http://purl.org/tio/ns#Event"/>
                    <rdf:Description rdf:about="http://purl.org/tio/ns#POI"/>
                    <rdf:Description rdf:about="http://purl.org/tio/ns#TransportationService"/>
                </owl:unionOf>
            </owl:Class>
        </rdfs:range>
        <rdfs:comment xml:lang="en">This links a tio:Ticket or a tio:ScopeOfAccess node to the tio:POI, tio:Event, or tio:TransportationService for which the tio:Ticket grants access.

Note: When used to link a tio:Ticket directly to a tio:POI, tio:Event, or tio:TransportationService, you cannot specify the various details of a tio:ScopeOfAccess node.</rdfs:comment>
        <rdfs:isDefinedBy rdf:resource="http://purl.org/tio/ns#"/>
        <rdfs:label xml:lang="en">accessTo (0..*)</rdfs:label>
    </owl:ObjectProperty>
    


    <!-- http://purl.org/tio/ns#ageRange -->

    <owl:ObjectProperty rdf:about="http://purl.org/tio/ns#ageRange">
        <rdfs:domain rdf:resource="http://purl.org/tio/ns#ScopeOfAccess"/>
        <rdfs:range rdf:resource="http://purl.org/goodrelations/v1#QuantitativeValue"/>
        <rdfs:comment xml:lang="en">The eligible age range or age ranges for admission to the revent, POI, or transportation service
Typical unit code(s): ANN for year (less frequently used: MON for months, WEE for weeks)</rdfs:comment>
        <rdfs:isDefinedBy rdf:resource="http://purl.org/tio/ns#"/>
        <rdfs:label xml:lang="en">ageRange (0..*)</rdfs:label>
    </owl:ObjectProperty>
    


    <!-- http://purl.org/tio/ns#at -->

    <owl:ObjectProperty rdf:about="http://purl.org/tio/ns#at">
        <rdfs:domain rdf:resource="http://purl.org/tio/ns#Stop"/>
        <rdfs:range rdf:resource="http://purl.org/tio/ns#POI"/>
        <rdfs:comment xml:lang="en">This indicates the location of a tio:Stop.</rdfs:comment>
        <rdfs:isDefinedBy rdf:resource="http://purl.org/tio/ns#"/>
        <rdfs:label xml:lang="en">at (1..1)</rdfs:label>
    </owl:ObjectProperty>
    


    <!-- http://purl.org/tio/ns#availableLayouts -->

    <owl:ObjectProperty rdf:about="http://purl.org/tio/ns#availableLayouts">
        <rdfs:domain rdf:resource="http://purl.org/tio/ns#POI"/>
        <rdfs:range rdf:resource="http://purl.org/tio/ns#SeatingLayout"/>
        <rdfs:comment xml:lang="en">This indicates the available seating layouts for a tio:POI.</rdfs:comment>
        <rdfs:isDefinedBy rdf:resource="http://purl.org/tio/ns#"/>
        <rdfs:label xml:lang="en">availableLayouts (0..*)</rdfs:label>
    </owl:ObjectProperty>
    


    <!-- http://purl.org/tio/ns#availableSeats -->

    <owl:ObjectProperty rdf:about="http://purl.org/tio/ns#availableSeats">
        <rdfs:domain rdf:resource="http://purl.org/tio/ns#SeatingLayout"/>
        <rdfs:range rdf:resource="http://purl.org/tio/ns#SeatOrSeatCategory"/>
        <rdfs:comment xml:lang="en">This indicates the individual seats for a given seating layout.</rdfs:comment>
        <rdfs:isDefinedBy rdf:resource="http://purl.org/tio/ns#"/>
        <rdfs:label xml:lang="en">availableSeats (0..*)</rdfs:label>
    </owl:ObjectProperty>
    


    <!-- http://purl.org/tio/ns#availableServiceLevel -->

    <owl:ObjectProperty rdf:about="http://purl.org/tio/ns#availableServiceLevel">
        <rdfs:subPropertyOf rdf:resource="http://purl.org/goodrelations/v1#qualitativeProductOrServiceProperty"/>
        <rdfs:domain rdf:resource="http://purl.org/tio/ns#TransportationService"/>
        <rdfs:range rdf:resource="http://purl.org/tio/ns#ServiceLevel"/>
        <rdfs:comment xml:lang="en">This indicates the service level(s) or fare class(es) available for the particular tio:TransportationService.</rdfs:comment>
        <rdfs:isDefinedBy rdf:resource="http://purl.org/tio/ns#"/>
        <rdfs:label xml:lang="en">availableServiceLevel (0..*)</rdfs:label>
    </owl:ObjectProperty>
    


    <!-- http://purl.org/tio/ns#durationOfAccess -->

    <owl:ObjectProperty rdf:about="http://purl.org/tio/ns#durationOfAccess">
        <rdfs:domain rdf:resource="http://purl.org/tio/ns#ScopeOfAccess"/>
        <rdfs:range rdf:resource="http://purl.org/goodrelations/v1#QuantitativeValue"/>
        <rdfs:comment xml:lang="en">The eligible duration of uninterrupted attendance or access.
Typical unit code(s): HUR for hours, DAY for days, WEE for weeks, MON for months, ANN for years </rdfs:comment>
        <rdfs:isDefinedBy rdf:resource="http://purl.org/tio/ns#"/>
        <rdfs:label xml:lang="en">durationOfAccess (0..1)</rdfs:label>
    </owl:ObjectProperty>
    


    <!-- http://purl.org/tio/ns#eligibleAudience -->

    <owl:ObjectProperty rdf:about="http://purl.org/tio/ns#eligibleAudience">
        <rdfs:domain rdf:resource="http://purl.org/tio/ns#ScopeOfAccess"/>
        <rdfs:range rdf:resource="http://purl.org/tio/ns#DiscountType"/>
        <rdfs:comment xml:lang="en">This links a tio:ScopeOfAccess node to the tio:DiscountType for which the specified access is granted.</rdfs:comment>
        <rdfs:isDefinedBy rdf:resource="http://purl.org/tio/ns#"/>
        <rdfs:label xml:lang="en">eligibleAudience (0..*)</rdfs:label>
    </owl:ObjectProperty>
    


    <!-- http://purl.org/tio/ns#eligibleServiceLevel -->

    <owl:ObjectProperty rdf:about="http://purl.org/tio/ns#eligibleServiceLevel">
        <rdfs:domain rdf:resource="http://purl.org/tio/ns#ScopeOfAccess"/>
        <rdfs:range rdf:resource="http://purl.org/tio/ns#ServiceLevel"/>
        <rdfs:comment xml:lang="en">This indicates the service level(s) or fare class(es) to which the tio:Ticket entitles.</rdfs:comment>
        <rdfs:isDefinedBy rdf:resource="http://purl.org/tio/ns#"/>
        <rdfs:label xml:lang="en">eligibleServiceLevel (0..*)</rdfs:label>
    </owl:ObjectProperty>
    


    <!-- http://purl.org/tio/ns#eligibleTimes -->

    <owl:ObjectProperty rdf:about="http://purl.org/tio/ns#eligibleTimes">
        <rdfs:domain rdf:resource="http://purl.org/tio/ns#ScopeOfAccess"/>
        <rdfs:range rdf:resource="http://purl.org/goodrelations/v1#OpeningHoursSpecification"/>
        <rdfs:comment xml:lang="en">This links a tio:ScopeOfAccess node to one or more gr:OpeningHoursSpecifications that indicate the times of access.

Note: The times of access for a particular ticket may be more constrained than the opening hours of the location, event, or transportation service. Use tio:openingHours for specifying the overall opening hours or hours of operation.</rdfs:comment>
        <rdfs:isDefinedBy rdf:resource="http://purl.org/tio/ns#"/>
        <rdfs:label xml:lang="en">eligibleTimes (0..*)</rdfs:label>
    </owl:ObjectProperty>
    


    <!-- http://purl.org/tio/ns#from -->

    <owl:ObjectProperty rdf:about="http://purl.org/tio/ns#from">
        <rdfs:domain rdf:resource="http://purl.org/tio/ns#TransportationService"/>
        <rdfs:range>
            <owl:Class>
                <owl:unionOf rdf:parseType="Collection">
                    <rdf:Description rdf:about="http://purl.org/tio/ns#POI"/>
                    <rdf:Description rdf:about="http://purl.org/tio/ns#Stop"/>
                </owl:unionOf>
            </owl:Class>
        </rdfs:range>
        <rdfs:comment xml:lang="en">This indicates the location of origin and time of departure.

Note: When the object of the statement is a tio:Stop, one can indicate the exact date and time for a single connection.
If such a level of detail is not needed, you can directly link to a point of interest, e.g. an instance of tio:POI.</rdfs:comment>
        <rdfs:isDefinedBy rdf:resource="http://purl.org/tio/ns#"/>
        <rdfs:label xml:lang="en">from (1..1)</rdfs:label>
    </owl:ObjectProperty>
    


    <!-- http://purl.org/tio/ns#includes -->

    <owl:ObjectProperty rdf:about="http://purl.org/tio/ns#includes">
        <rdf:type rdf:resource="http://www.w3.org/2002/07/owl#TransitiveProperty"/>
        <rdfs:domain rdf:resource="http://purl.org/tio/ns#POI"/>
        <rdfs:range rdf:resource="http://purl.org/tio/ns#POI"/>
        <rdfs:comment xml:lang="en">This indicates that a particular area includes another area or points of interest.

Note: Modeling geo-spatial relationships is non-trivial. This property is a very simple approach, sufficient for e.g. grouping all train stations in a particular fare area.</rdfs:comment>
        <rdfs:isDefinedBy rdf:resource="http://purl.org/tio/ns#"/>
        <rdfs:label xml:lang="en">includes (0..*)</rdfs:label>
    </owl:ObjectProperty>
    


    <!-- http://purl.org/tio/ns#noOfEntrances -->

    <owl:ObjectProperty rdf:about="http://purl.org/tio/ns#noOfEntrances">
        <rdfs:domain rdf:resource="http://purl.org/tio/ns#ScopeOfAccess"/>
        <rdfs:range rdf:resource="http://purl.org/goodrelations/v1#QuantitativeValueInteger"/>
        <rdfs:comment xml:lang="en">The number of times the respective participant(s) is/are allowed to enter the event, POI, or transportation service
Typical unit code(s): C62 for times </rdfs:comment>
        <rdfs:isDefinedBy rdf:resource="http://purl.org/tio/ns#"/>
        <rdfs:label xml:lang="en">noOfEntrances (0..1)</rdfs:label>
    </owl:ObjectProperty>
    


    <!-- http://purl.org/tio/ns#openingHours -->

    <owl:ObjectProperty rdf:about="http://purl.org/tio/ns#openingHours">
        <rdfs:domain rdf:resource="http://purl.org/tio/ns#POI"/>
        <rdfs:range rdf:resource="http://purl.org/goodrelations/v1#OpeningHoursSpecification"/>
        <rdfs:comment xml:lang="en">This indicates the opening hours for a point of interest. 

Note: The opening hours of the location and the time-windows for which a particular ticket is eligible may differ. Use tio:eligibleTimes for the latter.</rdfs:comment>
        <rdfs:isDefinedBy rdf:resource="http://purl.org/tio/ns#"/>
        <rdfs:label xml:lang="en">openingHours (0..*)</rdfs:label>
    </owl:ObjectProperty>
    


    <!-- http://purl.org/tio/ns#operatedBy -->

    <owl:ObjectProperty rdf:about="http://purl.org/tio/ns#operatedBy">
        <rdfs:domain rdf:resource="http://purl.org/tio/ns#TransportationService"/>
        <rdfs:range rdf:resource="http://purl.org/goodrelations/v1#BusinessEntity"/>
        <rdfs:comment xml:lang="en">This indicates the business entity that actually operates the vessel used for a transportation service.</rdfs:comment>
        <rdfs:isDefinedBy rdf:resource="http://purl.org/tio/ns#"/>
        <rdfs:label xml:lang="en">operatedBy (0..1)</rdfs:label>
    </owl:ObjectProperty>
    


    <!-- http://purl.org/tio/ns#participants -->

    <owl:ObjectProperty rdf:about="http://purl.org/tio/ns#participants">
        <rdfs:domain rdf:resource="http://purl.org/tio/ns#ScopeOfAccess"/>
        <rdfs:range rdf:resource="http://purl.org/goodrelations/v1#QuantitativeValueInteger"/>
        <rdfs:comment xml:lang="en">The number of participants that are allowed to enter the event, POI, or use transportation service
Typical unit code(s): C62 for persons </rdfs:comment>
        <rdfs:isDefinedBy rdf:resource="http://purl.org/tio/ns#"/>
        <rdfs:label xml:lang="en">participants (0..1)</rdfs:label>
    </owl:ObjectProperty>
    


    <!-- http://purl.org/tio/ns#scope -->

    <owl:ObjectProperty rdf:about="http://purl.org/tio/ns#scope">
        <rdfs:domain rdf:resource="http://purl.org/tio/ns#Ticket"/>
        <rdfs:range rdf:resource="http://purl.org/tio/ns#ScopeOfAccess"/>
        <rdfs:comment xml:lang="en">This links a tio:Ticket to the tio:ScopeOfAccess node or nodes that are included in the ticket. 

Note: For simple scenarios, you can also directly use tio:accessTo.</rdfs:comment>
        <rdfs:isDefinedBy rdf:resource="http://purl.org/tio/ns#"/>
        <rdfs:label xml:lang="en">scope (0..*)</rdfs:label>
    </owl:ObjectProperty>
    


    <!-- http://purl.org/tio/ns#seat -->

    <owl:ObjectProperty rdf:about="http://purl.org/tio/ns#seat">
        <rdfs:domain rdf:resource="http://purl.org/tio/ns#ScopeOfAccess"/>
        <rdfs:range rdf:resource="http://purl.org/tio/ns#SeatOrSeatCategory"/>
        <rdfs:comment xml:lang="en">This indicates the seat or seat category.</rdfs:comment>
        <rdfs:isDefinedBy rdf:resource="http://purl.org/tio/ns#"/>
        <rdfs:label xml:lang="en">seat (0..*)</rdfs:label>
    </owl:ObjectProperty>
    


    <!-- http://purl.org/tio/ns#takesPlaceAt -->

    <owl:ObjectProperty rdf:about="http://purl.org/tio/ns#takesPlaceAt">
        <rdfs:domain rdf:resource="http://purl.org/tio/ns#Event"/>
        <rdfs:range rdf:resource="http://purl.org/tio/ns#POI"/>
        <rdfs:comment xml:lang="en">This indicates the location or locations of a tio:Event.</rdfs:comment>
        <rdfs:isDefinedBy rdf:resource="http://purl.org/tio/ns#"/>
        <rdfs:label xml:lang="en">takesPlaceAt (0..*)</rdfs:label>
    </owl:ObjectProperty>
    


    <!-- http://purl.org/tio/ns#to -->

    <owl:ObjectProperty rdf:about="http://purl.org/tio/ns#to">
        <rdfs:domain rdf:resource="http://purl.org/tio/ns#TransportationService"/>
        <rdfs:range>
            <owl:Class>
                <owl:unionOf rdf:parseType="Collection">
                    <rdf:Description rdf:about="http://purl.org/tio/ns#POI"/>
                    <rdf:Description rdf:about="http://purl.org/tio/ns#Stop"/>
                </owl:unionOf>
            </owl:Class>
        </rdfs:range>
        <rdfs:comment xml:lang="en">This indicates the destination and time of arrival.

Note: When the object of the statement is a tio:Stop, one can indicate the exact date and time for a single connection.
If such a level of detail is not needed, you can directly link to a point of interest, e.g. an instance of tio:POI.</rdfs:comment>
        <rdfs:isDefinedBy rdf:resource="http://purl.org/tio/ns#"/>
        <rdfs:label xml:lang="en">to (1..1)</rdfs:label>
    </owl:ObjectProperty>
    


    <!-- http://purl.org/tio/ns#via -->

    <owl:ObjectProperty rdf:about="http://purl.org/tio/ns#via">
        <rdfs:domain rdf:resource="http://purl.org/tio/ns#TransportationService"/>
        <rdfs:range>
            <owl:Class>
                <owl:unionOf rdf:parseType="Collection">
                    <rdf:Description rdf:about="http://purl.org/tio/ns#POI"/>
                    <rdf:Description rdf:about="http://purl.org/tio/ns#Stop"/>
                </owl:unionOf>
            </owl:Class>
        </rdfs:range>
        <rdfs:comment xml:lang="en">This indicates the location, time of arrival, and time of departure for an intermediate stop.

Note: When the object of the statement is a tio:Stop, one can indicate the exact date and time for a single connection.
If such a level of detail is not needed, you can directly link to a point of interest, e.g. an instance of tio:POI.</rdfs:comment>
        <rdfs:isDefinedBy rdf:resource="http://purl.org/tio/ns#"/>
        <rdfs:label xml:lang="en">via (0..*)</rdfs:label>
    </owl:ObjectProperty>
    


    <!-- 
    ///////////////////////////////////////////////////////////////////////////////////////
    //
    // Data properties
    //
    ///////////////////////////////////////////////////////////////////////////////////////
     -->

    


    <!-- http://purl.org/tio/ns#arrives -->

    <owl:DatatypeProperty rdf:about="http://purl.org/tio/ns#arrives">
        <rdfs:domain rdf:resource="http://purl.org/tio/ns#Stop"/>
        <rdfs:range rdf:resource="http://www.w3.org/2001/XMLSchema#dateTime"/>
        <rdfs:comment xml:lang="en">The date and time at which the transportation service will arrive at the respective tio:Stop</rdfs:comment>
        <rdfs:isDefinedBy rdf:resource="http://purl.org/tio/ns#"/>
        <rdfs:label xml:lang="en">arrives (0..1)</rdfs:label>
    </owl:DatatypeProperty>
    


    <!-- http://purl.org/tio/ns#available -->

    <owl:DatatypeProperty rdf:about="http://purl.org/tio/ns#available">
        <rdfs:domain rdf:resource="http://purl.org/tio/ns#TicketPlaceholder"/>
        <rdfs:range rdf:resource="http://www.w3.org/2001/XMLSchema#integer"/>
        <rdfs:comment xml:lang="en">The number of tickets of this category still available at the time of publishing the data</rdfs:comment>
        <rdfs:isDefinedBy rdf:resource="http://purl.org/tio/ns#"/>
        <rdfs:label xml:lang="en">available (0..1)</rdfs:label>
    </owl:DatatypeProperty>
    


    <!-- http://purl.org/tio/ns#departs -->

    <owl:DatatypeProperty rdf:about="http://purl.org/tio/ns#departs">
        <rdfs:domain rdf:resource="http://purl.org/tio/ns#Stop"/>
        <rdfs:range rdf:resource="http://www.w3.org/2001/XMLSchema#dateTime"/>
        <rdfs:comment xml:lang="en">The date and time at which the transportation service will depart from the respective tio:Stop</rdfs:comment>
        <rdfs:isDefinedBy rdf:resource="http://purl.org/tio/ns#"/>
        <rdfs:label xml:lang="en">departs (0..1)</rdfs:label>
    </owl:DatatypeProperty>
    


    <!-- http://purl.org/tio/ns#ends -->

    <owl:DatatypeProperty rdf:about="http://purl.org/tio/ns#ends">
        <rdfs:domain rdf:resource="http://purl.org/tio/ns#Event"/>
        <rdfs:range rdf:resource="http://www.w3.org/2001/XMLSchema#dateTime"/>
        <rdfs:comment xml:lang="en">The date and time for which the event is scheduled to end

Note: You can attach the time and date of the event using tio:starts and tio:ends as simple datatype properties,
even if lode:Event and event:Event recommend other, more sophisticated ways of modeling the temporal aspects of events.</rdfs:comment>
        <rdfs:isDefinedBy rdf:resource="http://purl.org/tio/ns#"/>
        <rdfs:label xml:lang="en">ends (0..1)</rdfs:label>
    </owl:DatatypeProperty>
    


    <!-- http://purl.org/tio/ns#flightNo -->

    <owl:DatatypeProperty rdf:about="http://purl.org/tio/ns#flightNo">
        <rdfs:domain rdf:resource="http://purl.org/tio/ns#Flight"/>
        <rdfs:range rdf:resource="http://www.w3.org/2001/XMLSchema#string"/>
        <rdfs:comment xml:lang="en">The flight number (or numbers, in case of codeshare flights)</rdfs:comment>
        <rdfs:isDefinedBy rdf:resource="http://purl.org/tio/ns#"/>
        <rdfs:label xml:lang="en">flightNo (0..*)</rdfs:label>
    </owl:DatatypeProperty>
    


    <!-- http://purl.org/tio/ns#sold -->

    <owl:DatatypeProperty rdf:about="http://purl.org/tio/ns#sold">
        <rdfs:domain rdf:resource="http://purl.org/tio/ns#TicketPlaceholder"/>
        <rdfs:range rdf:resource="http://www.w3.org/2001/XMLSchema#integer"/>
        <rdfs:comment xml:lang="en">The number of tickets of this category already sold at the time of publishing the data</rdfs:comment>
        <rdfs:isDefinedBy rdf:resource="http://purl.org/tio/ns#"/>
        <rdfs:label xml:lang="en">sold (0..1)</rdfs:label>
    </owl:DatatypeProperty>
    


    <!-- http://purl.org/tio/ns#starts -->

    <owl:DatatypeProperty rdf:about="http://purl.org/tio/ns#starts">
        <rdfs:domain rdf:resource="http://purl.org/tio/ns#Event"/>
        <rdfs:range rdf:resource="http://www.w3.org/2001/XMLSchema#dateTime"/>
        <rdfs:comment xml:lang="en">The date and time for which the event is scheduled to begin

Note: You can attach the time and date of the event using tio:starts and tio:ends as simple datatype properties,
even if lode:Event and event:Event recommend other, more sophisticated ways of modeling the temporal aspects of events.</rdfs:comment>
        <rdfs:isDefinedBy rdf:resource="http://purl.org/tio/ns#"/>
        <rdfs:label xml:lang="en">starts (0..1)</rdfs:label>
    </owl:DatatypeProperty>
    


    <!-- http://purl.org/tio/ns#ticketID -->

    <owl:DatatypeProperty rdf:about="http://purl.org/tio/ns#ticketID">
        <rdfs:subPropertyOf rdf:resource="http://purl.org/goodrelations/v1#datatypeProductOrServiceProperty"/>
        <rdfs:domain rdf:resource="http://purl.org/tio/ns#Ticket"/>
        <rdfs:range rdf:resource="http://www.w3.org/2001/XMLSchema#string"/>
        <rdfs:comment xml:lang="en">A unique identifier for a particular ticket or ticket type.</rdfs:comment>
        <rdfs:isDefinedBy rdf:resource="http://purl.org/tio/ns#"/>
        <rdfs:label xml:lang="en">ticketID (0..1)</rdfs:label>
    </owl:DatatypeProperty>
    


    <!-- http://purl.org/tio/ns#total -->

    <owl:DatatypeProperty rdf:about="http://purl.org/tio/ns#total">
        <rdfs:domain rdf:resource="http://purl.org/tio/ns#TicketPlaceholder"/>
        <rdfs:range rdf:resource="http://www.w3.org/2001/XMLSchema#integer"/>
        <rdfs:comment xml:lang="en">The total number of tickets of this category that will be issued for the event</rdfs:comment>
        <rdfs:isDefinedBy rdf:resource="http://purl.org/tio/ns#"/>
        <rdfs:label xml:lang="en">total (0..1)</rdfs:label>
    </owl:DatatypeProperty>
    


    <!-- http://purl.org/tio/ns#validFrom -->

    <owl:DatatypeProperty rdf:about="http://purl.org/tio/ns#validFrom">
        <rdfs:domain>
            <owl:Class>
                <owl:unionOf rdf:parseType="Collection">
                    <rdf:Description rdf:about="http://purl.org/tio/ns#ScopeOfAccess"/>
                    <rdf:Description rdf:about="http://purl.org/tio/ns#Ticket"/>
                </owl:unionOf>
            </owl:Class>
        </rdfs:domain>
        <rdfs:range rdf:resource="http://www.w3.org/2001/XMLSchema#dateTime"/>
        <rdfs:comment xml:lang="en">This property specifies the beginning of the validity of the access or right that the ticket grants. 
It can be attached to the tio:Ticket (if meant for the ticket as a whole) and to individual tio:ScopeOfAccess entities (if meant for just a particular part of the access rights).

A time-zone should be specified. For a time in GMT/UTC, simply add a &quot;Z&quot; following the time:

2010-11-15T09:30:10Z.

Alternatively, you can specify an offset from the UTC time by adding a positive or negative time following the time:

2010-11-15T09:30:10-09:00

or

2010-11-15T09:30:10+09:00.</rdfs:comment>
        <rdfs:isDefinedBy rdf:resource="http://purl.org/tio/ns#"/>
        <rdfs:label xml:lang="en">validFrom (0..1)</rdfs:label>
    </owl:DatatypeProperty>
    


    <!-- http://purl.org/tio/ns#validThrough -->

    <owl:DatatypeProperty rdf:about="http://purl.org/tio/ns#validThrough">
        <rdfs:domain>
            <owl:Class>
                <owl:unionOf rdf:parseType="Collection">
                    <rdf:Description rdf:about="http://purl.org/tio/ns#ScopeOfAccess"/>
                    <rdf:Description rdf:about="http://purl.org/tio/ns#Ticket"/>
                </owl:unionOf>
            </owl:Class>
        </rdfs:domain>
        <rdfs:range rdf:resource="http://www.w3.org/2001/XMLSchema#dateTime"/>
        <rdfs:comment xml:lang="en">This property specifies the ending of the validity of the access or right that the ticket grants. 
It can be attached to the tio:Ticket (if meant for the ticket as a whole) and to individual tio:ScopeOfAccess entities (if meant for just a particular part of the access rights).

A time-zone should be specified. For a time in GMT/UTC, simply add a &quot;Z&quot; following the time:

2010-11-15T09:30:10Z.

Alternatively, you can specify an offset from the UTC time by adding a positive or negative time following the time:

2010-11-15T09:30:10-09:00

or

2010-11-15T09:30:10+09:00.</rdfs:comment>
        <rdfs:isDefinedBy rdf:resource="http://purl.org/tio/ns#"/>
        <rdfs:label xml:lang="en">validThrough (0..1)</rdfs:label>
    </owl:DatatypeProperty>
    


    <!-- 
    ///////////////////////////////////////////////////////////////////////////////////////
    //
    // Classes
    //
    ///////////////////////////////////////////////////////////////////////////////////////
     -->

    


    <!-- http://linkedevents.org/ontology/Event -->

    <owl:Class rdf:about="http://linkedevents.org/ontology/Event"/>
    


    <!-- http://purl.org/NET/c4dm/event.owl#Event -->

    <owl:Class rdf:about="http://purl.org/NET/c4dm/event.owl#Event"/>
    


    <!-- http://purl.org/goodrelations/v1#BusinessEntity -->

    <rdf:Description rdf:about="http://purl.org/goodrelations/v1#BusinessEntity">
        <owl:disjointWith rdf:resource="http://purl.org/tio/ns#Event"/>
        <owl:disjointWith rdf:resource="http://purl.org/tio/ns#ScopeOfAccess"/>
        <owl:disjointWith rdf:resource="http://purl.org/tio/ns#SeatingLayout"/>
        <owl:disjointWith rdf:resource="http://purl.org/tio/ns#Stop"/>
    </rdf:Description>
    


    <!-- http://purl.org/goodrelations/v1#BusinessEntityType -->

    <rdf:Description rdf:about="http://purl.org/goodrelations/v1#BusinessEntityType">
        <owl:disjointWith rdf:resource="http://purl.org/tio/ns#Event"/>
        <owl:disjointWith rdf:resource="http://purl.org/tio/ns#ScopeOfAccess"/>
        <owl:disjointWith rdf:resource="http://purl.org/tio/ns#SeatingLayout"/>
        <owl:disjointWith rdf:resource="http://purl.org/tio/ns#Stop"/>
    </rdf:Description>
    


    <!-- http://purl.org/goodrelations/v1#BusinessFunction -->

    <rdf:Description rdf:about="http://purl.org/goodrelations/v1#BusinessFunction">
        <owl:disjointWith rdf:resource="http://purl.org/tio/ns#Event"/>
        <owl:disjointWith rdf:resource="http://purl.org/tio/ns#ScopeOfAccess"/>
        <owl:disjointWith rdf:resource="http://purl.org/tio/ns#SeatingLayout"/>
        <owl:disjointWith rdf:resource="http://purl.org/tio/ns#Stop"/>
    </rdf:Description>
    


    <!-- http://purl.org/goodrelations/v1#DayOfWeek -->

    <rdf:Description rdf:about="http://purl.org/goodrelations/v1#DayOfWeek">
        <owl:disjointWith rdf:resource="http://purl.org/tio/ns#Event"/>
        <owl:disjointWith rdf:resource="http://purl.org/tio/ns#ScopeOfAccess"/>
        <owl:disjointWith rdf:resource="http://purl.org/tio/ns#SeatingLayout"/>
        <owl:disjointWith rdf:resource="http://purl.org/tio/ns#Stop"/>
    </rdf:Description>
    


    <!-- http://purl.org/goodrelations/v1#DeliveryMethod -->

    <rdf:Description rdf:about="http://purl.org/goodrelations/v1#DeliveryMethod">
        <owl:disjointWith rdf:resource="http://purl.org/tio/ns#Event"/>
        <owl:disjointWith rdf:resource="http://purl.org/tio/ns#ScopeOfAccess"/>
        <owl:disjointWith rdf:resource="http://purl.org/tio/ns#SeatingLayout"/>
        <owl:disjointWith rdf:resource="http://purl.org/tio/ns#Stop"/>
    </rdf:Description>
    


    <!-- http://purl.org/goodrelations/v1#LocationOfSalesOrServiceProvisioning -->

    <rdf:Description rdf:about="http://purl.org/goodrelations/v1#LocationOfSalesOrServiceProvisioning">
        <owl:disjointWith rdf:resource="http://purl.org/tio/ns#Event"/>
        <owl:disjointWith rdf:resource="http://purl.org/tio/ns#ScopeOfAccess"/>
        <owl:disjointWith rdf:resource="http://purl.org/tio/ns#SeatingLayout"/>
        <owl:disjointWith rdf:resource="http://purl.org/tio/ns#Stop"/>
    </rdf:Description>
    


    <!-- http://purl.org/goodrelations/v1#N-Ary-Relations -->

    <rdf:Description rdf:about="http://purl.org/goodrelations/v1#N-Ary-Relations">
        <owl:disjointWith rdf:resource="http://purl.org/tio/ns#Event"/>
        <owl:disjointWith rdf:resource="http://purl.org/tio/ns#ScopeOfAccess"/>
        <owl:disjointWith rdf:resource="http://purl.org/tio/ns#SeatingLayout"/>
        <owl:disjointWith rdf:resource="http://purl.org/tio/ns#Stop"/>
    </rdf:Description>
    


    <!-- http://purl.org/goodrelations/v1#Offering -->

    <rdf:Description rdf:about="http://purl.org/goodrelations/v1#Offering">
        <owl:disjointWith rdf:resource="http://purl.org/tio/ns#Event"/>
        <owl:disjointWith rdf:resource="http://purl.org/tio/ns#ScopeOfAccess"/>
        <owl:disjointWith rdf:resource="http://purl.org/tio/ns#SeatingLayout"/>
        <owl:disjointWith rdf:resource="http://purl.org/tio/ns#Stop"/>
    </rdf:Description>
    


    <!-- http://purl.org/goodrelations/v1#PaymentMethod -->

    <rdf:Description rdf:about="http://purl.org/goodrelations/v1#PaymentMethod">
        <owl:disjointWith rdf:resource="http://purl.org/tio/ns#Event"/>
        <owl:disjointWith rdf:resource="http://purl.org/tio/ns#ScopeOfAccess"/>
        <owl:disjointWith rdf:resource="http://purl.org/tio/ns#SeatingLayout"/>
        <owl:disjointWith rdf:resource="http://purl.org/tio/ns#Stop"/>
    </rdf:Description>
    


    <!-- http://purl.org/goodrelations/v1#PriceSpecification -->

    <rdf:Description rdf:about="http://purl.org/goodrelations/v1#PriceSpecification">
        <owl:disjointWith rdf:resource="http://purl.org/tio/ns#Event"/>
        <owl:disjointWith rdf:resource="http://purl.org/tio/ns#ScopeOfAccess"/>
        <owl:disjointWith rdf:resource="http://purl.org/tio/ns#SeatingLayout"/>
        <owl:disjointWith rdf:resource="http://purl.org/tio/ns#Stop"/>
    </rdf:Description>
    


    <!-- http://purl.org/goodrelations/v1#ProductOrService -->

    <rdf:Description rdf:about="http://purl.org/goodrelations/v1#ProductOrService">
        <owl:disjointWith rdf:resource="http://purl.org/tio/ns#Event"/>
        <owl:disjointWith rdf:resource="http://purl.org/tio/ns#ScopeOfAccess"/>
        <owl:disjointWith rdf:resource="http://purl.org/tio/ns#SeatingLayout"/>
        <owl:disjointWith rdf:resource="http://purl.org/tio/ns#Stop"/>
    </rdf:Description>
    


    <!-- http://purl.org/goodrelations/v1#QualitativeValue -->

    <rdf:Description rdf:about="http://purl.org/goodrelations/v1#QualitativeValue">
        <owl:disjointWith rdf:resource="http://purl.org/tio/ns#Event"/>
        <owl:disjointWith rdf:resource="http://purl.org/tio/ns#ScopeOfAccess"/>
        <owl:disjointWith rdf:resource="http://purl.org/tio/ns#SeatingLayout"/>
        <owl:disjointWith rdf:resource="http://purl.org/tio/ns#Stop"/>
    </rdf:Description>
    


    <!-- http://purl.org/goodrelations/v1#QuantitativeValue -->

    <rdf:Description rdf:about="http://purl.org/goodrelations/v1#QuantitativeValue">
        <owl:disjointWith rdf:resource="http://purl.org/tio/ns#Event"/>
        <owl:disjointWith rdf:resource="http://purl.org/tio/ns#ScopeOfAccess"/>
        <owl:disjointWith rdf:resource="http://purl.org/tio/ns#SeatingLayout"/>
        <owl:disjointWith rdf:resource="http://purl.org/tio/ns#Stop"/>
    </rdf:Description>
    


    <!-- http://purl.org/goodrelations/v1#WarrantyScope -->

    <rdf:Description rdf:about="http://purl.org/goodrelations/v1#WarrantyScope">
        <owl:disjointWith rdf:resource="http://purl.org/tio/ns#Event"/>
        <owl:disjointWith rdf:resource="http://purl.org/tio/ns#ScopeOfAccess"/>
        <owl:disjointWith rdf:resource="http://purl.org/tio/ns#SeatingLayout"/>
        <owl:disjointWith rdf:resource="http://purl.org/tio/ns#Stop"/>
    </rdf:Description>
    


    <!-- http://purl.org/tio/ns#ActualTicket -->

    <owl:Class rdf:about="http://purl.org/tio/ns#ActualTicket">
        <rdfs:subClassOf rdf:resource="http://purl.org/goodrelations/v1#ActualProductOrServiceInstance"/>
        <rdfs:subClassOf rdf:resource="http://purl.org/tio/ns#Ticket"/>
        <owl:disjointWith rdf:resource="http://purl.org/tio/ns#TicketPlaceholder"/>
        <rdfs:comment xml:lang="en">An actual ticket is single, identifiable right to access a particular event, location, or transportation service.</rdfs:comment>
        <rdfs:isDefinedBy rdf:resource="http://purl.org/tio/ns#"/>
        <rdfs:label xml:lang="en">ActualTicket (gr:ProductOrService)</rdfs:label>
    </owl:Class>
    


    <!-- http://purl.org/tio/ns#CoachService -->

    <owl:Class rdf:about="http://purl.org/tio/ns#CoachService">
        <rdfs:subClassOf rdf:resource="http://purl.org/tio/ns#TransportationService"/>
        <owl:disjointWith rdf:resource="http://purl.org/tio/ns#Flight"/>
        <owl:disjointWith rdf:resource="http://purl.org/tio/ns#Taxi"/>
        <owl:disjointWith rdf:resource="http://purl.org/tio/ns#TrainService"/>
        <rdfs:comment xml:lang="en">A regular or individual service to transport passengers or cargo from one location to another location by means of a coach or bus.</rdfs:comment>
        <rdfs:isDefinedBy rdf:resource="http://purl.org/tio/ns#"/>
        <rdfs:label xml:lang="en">CoachService</rdfs:label>
    </owl:Class>
    


    <!-- http://purl.org/tio/ns#DiscountType -->

    <owl:Class rdf:about="http://purl.org/tio/ns#DiscountType">
        <rdfs:subClassOf rdf:resource="http://purl.org/goodrelations/v1#QualitativeValue"/>
        <owl:disjointWith rdf:resource="http://purl.org/tio/ns#Event"/>
        <owl:disjointWith rdf:resource="http://purl.org/tio/ns#ScopeOfAccess"/>
        <owl:disjointWith rdf:resource="http://purl.org/tio/ns#SeatingLayout"/>
        <owl:disjointWith rdf:resource="http://purl.org/tio/ns#Stop"/>
        <rdfs:comment xml:lang="en">The class of qualitative values indicating a discount type, audience, or group type - e.g. students, military personnel, etc.

Note: Discount types that solely represent age ranges (e.g. children, senior citizens, ...) are better expressed using tio:ageRange.</rdfs:comment>
        <rdfs:isDefinedBy rdf:resource="http://purl.org/tio/ns#"/>
        <rdfs:label xml:lang="en">DiscountType (gr:QualitativeValue)</rdfs:label>
    </owl:Class>
    


    <!-- http://purl.org/tio/ns#Event -->

    <owl:Class rdf:about="http://purl.org/tio/ns#Event">
        <rdfs:subClassOf>
            <owl:Class>
                <owl:unionOf rdf:parseType="Collection">
                    <rdf:Description rdf:about="http://linkedevents.org/ontology/Event"/>
                    <rdf:Description rdf:about="http://purl.org/NET/c4dm/event.owl#Event"/>
                    <rdf:Description rdf:about="http://www.loa-cnr.it/ontologies/DUL.owl#Event"/>
                </owl:unionOf>
            </owl:Class>
        </rdfs:subClassOf>
        <owl:disjointWith rdf:resource="http://purl.org/tio/ns#POI"/>
        <owl:disjointWith rdf:resource="http://purl.org/tio/ns#ScopeOfAccess"/>
        <owl:disjointWith rdf:resource="http://purl.org/tio/ns#SeatOrSeatCategory"/>
        <owl:disjointWith rdf:resource="http://purl.org/tio/ns#SeatingLayout"/>
        <owl:disjointWith rdf:resource="http://purl.org/tio/ns#ServiceLevel"/>
        <owl:disjointWith rdf:resource="http://purl.org/tio/ns#Stop"/>
        <owl:disjointWith rdf:resource="http://purl.org/tio/ns#Ticket"/>
        <owl:disjointWith rdf:resource="http://purl.org/tio/ns#TransportationService"/>
        <rdfs:comment xml:lang="en">An event, e.g. a concert, a show, etc. You can also safely use the following external classes for describing the respective event:

http://linkedevents.org/ontology/Event (lode:Event)
http://purl.org/NET/c4dm/event.owl#Event (event:Event)
http://www.loa-cnr.it/ontologies/DUL.owl#Event (dul:Event)

Note: You can attach the time and date of the event using tio:starts and tio:ends as simple datatype properties, even if lode:Event and event:Event recommend other, more sophisticated ways of modeling the temporal aspects of events.</rdfs:comment>
        <rdfs:isDefinedBy rdf:resource="http://purl.org/tio/ns#"/>
        <rdfs:label xml:lang="en">Event</rdfs:label>
    </owl:Class>
    


    <!-- http://purl.org/tio/ns#Flight -->

    <owl:Class rdf:about="http://purl.org/tio/ns#Flight">
        <rdfs:subClassOf rdf:resource="http://purl.org/tio/ns#TransportationService"/>
        <owl:disjointWith rdf:resource="http://purl.org/tio/ns#Taxi"/>
        <owl:disjointWith rdf:resource="http://purl.org/tio/ns#TrainService"/>
        <rdfs:comment xml:lang="en">A regular or individual service to transport passengers or cargo from one location to another location by means of an aircraft

Note: By design, the Tickets Ontology does not provide mechanisms for modeling rules for recurring patterns of transportation services (e.g. every Monday at 8:00). Instead, it expects that you materialize each individual connection on a given day.
Most flight schedule applications are complex databases, so they will have to be exposed as SPARQL endpoints anyway.</rdfs:comment>
        <rdfs:isDefinedBy rdf:resource="http://purl.org/tio/ns#"/>
        <rdfs:label xml:lang="en">Flight</rdfs:label>
    </owl:Class>
    


    <!-- http://purl.org/tio/ns#POI -->

    <owl:Class rdf:about="http://purl.org/tio/ns#POI">
        <rdfs:subClassOf rdf:resource="http://purl.org/goodrelations/v1#LocationOfSalesOrServiceProvisioning"/>
        <owl:disjointWith rdf:resource="http://purl.org/tio/ns#ScopeOfAccess"/>
        <owl:disjointWith rdf:resource="http://purl.org/tio/ns#SeatingLayout"/>
        <owl:disjointWith rdf:resource="http://purl.org/tio/ns#Stop"/>
        <rdfs:comment xml:lang="en">A point or area of interest, e.g. a museum, a train station, an airport, a bus stop, a store, a box office, etc.

Note 1: Use existing vocabularies like vcard or geo to attach address and geoposition (lat/long) details to the location.
Note 2: You can safely re-use any existing location, area, or point of interest from other data sources, e.g. DBPedia.</rdfs:comment>
        <rdfs:isDefinedBy rdf:resource="http://purl.org/tio/ns#"/>
        <rdfs:label xml:lang="en">POI (gr:LocationOfSalesOrServiceProvisioning)</rdfs:label>
    </owl:Class>
    


    <!-- http://purl.org/tio/ns#ScopeOfAccess -->

    <owl:Class rdf:about="http://purl.org/tio/ns#ScopeOfAccess">
        <owl:disjointWith rdf:resource="http://purl.org/tio/ns#SeatOrSeatCategory"/>
        <owl:disjointWith rdf:resource="http://purl.org/tio/ns#SeatingLayout"/>
        <owl:disjointWith rdf:resource="http://purl.org/tio/ns#ServiceLevel"/>
        <owl:disjointWith rdf:resource="http://purl.org/tio/ns#Stop"/>
        <owl:disjointWith rdf:resource="http://purl.org/tio/ns#Ticket"/>
        <owl:disjointWith rdf:resource="http://purl.org/tio/ns#TransportationService"/>
        <rdfs:comment xml:lang="en">This is a conceptual entity that collates all properties defining the type of access a ticket provides to a particular event, location, or transportation.</rdfs:comment>
        <rdfs:isDefinedBy rdf:resource="http://purl.org/tio/ns#"/>
        <rdfs:label xml:lang="en">ScopeOfAccess</rdfs:label>
    </owl:Class>
    


    <!-- http://purl.org/tio/ns#SeatOrSeatCategory -->

    <owl:Class rdf:about="http://purl.org/tio/ns#SeatOrSeatCategory">
        <rdfs:subClassOf rdf:resource="http://purl.org/goodrelations/v1#QualitativeValue"/>
        <owl:disjointWith rdf:resource="http://purl.org/tio/ns#SeatingLayout"/>
        <owl:disjointWith rdf:resource="http://purl.org/tio/ns#Stop"/>
        <rdfs:comment xml:lang="en">The class of qualitative values indicating a seat position (e.g. the seat 4B in a given plane) or a seat category (e.g. window seat). 
    Note that the same vessel or building may have multiple seating layouts.</rdfs:comment>
        <rdfs:isDefinedBy rdf:resource="http://purl.org/tio/ns#"/>
        <rdfs:label xml:lang="en">SeatOrSeatCategory (gr:QualitativeValue)</rdfs:label>
    </owl:Class>
    


    <!-- http://purl.org/tio/ns#SeatingLayout -->

    <owl:Class rdf:about="http://purl.org/tio/ns#SeatingLayout">
        <owl:disjointWith rdf:resource="http://purl.org/tio/ns#ServiceLevel"/>
        <owl:disjointWith rdf:resource="http://purl.org/tio/ns#Stop"/>
        <owl:disjointWith rdf:resource="http://purl.org/tio/ns#Ticket"/>
        <owl:disjointWith rdf:resource="http://purl.org/tio/ns#TransportationService"/>
        <rdfs:comment xml:lang="en">A seating layout for a particular location, vessel, or single transportation service</rdfs:comment>
        <rdfs:isDefinedBy rdf:resource="http://purl.org/tio/ns#"/>
        <rdfs:label xml:lang="en">SeatingLayout</rdfs:label>
    </owl:Class>
    


    <!-- http://purl.org/tio/ns#ServiceLevel -->

    <owl:Class rdf:about="http://purl.org/tio/ns#ServiceLevel">
        <rdfs:subClassOf rdf:resource="http://purl.org/goodrelations/v1#QualitativeValue"/>
        <owl:disjointWith rdf:resource="http://purl.org/tio/ns#Stop"/>
        <rdfs:comment xml:lang="en">The class of qualitative values indicating a service level oder fare class (e.g. Business Class).</rdfs:comment>
        <rdfs:isDefinedBy rdf:resource="http://purl.org/tio/ns#"/>
        <rdfs:label xml:lang="en">ServiceLevel (gr:QualitativeValue)</rdfs:label>
    </owl:Class>
    


    <!-- http://purl.org/tio/ns#Stop -->

    <owl:Class rdf:about="http://purl.org/tio/ns#Stop">
        <owl:disjointWith rdf:resource="http://purl.org/tio/ns#Ticket"/>
        <owl:disjointWith rdf:resource="http://purl.org/tio/ns#TransportationService"/>
        <rdfs:comment xml:lang="en">The initial, final, or any intermediate point in time and space of a particular tio:TransportationService, 
characterized by its location (tio:at), arrival time (tio:arrives), and departure time (tio:departs). 
Each tio:TransportationService has at least one tio:Stop for the point and time of departure and another one for the final destination.</rdfs:comment>
        <rdfs:isDefinedBy rdf:resource="http://purl.org/tio/ns#"/>
        <rdfs:label xml:lang="en">Stop</rdfs:label>
    </owl:Class>
    


    <!-- http://purl.org/tio/ns#Taxi -->

    <owl:Class rdf:about="http://purl.org/tio/ns#Taxi">
        <rdfs:subClassOf rdf:resource="http://purl.org/tio/ns#TransportationService"/>
        <owl:disjointWith rdf:resource="http://purl.org/tio/ns#TrainService"/>
        <rdfs:comment xml:lang="en">A taxi service to transport passengers from one location to another location</rdfs:comment>
        <rdfs:isDefinedBy rdf:resource="http://purl.org/tio/ns#"/>
        <rdfs:label xml:lang="en">Taxi</rdfs:label>
    </owl:Class>
    


    <!-- http://purl.org/tio/ns#Ticket -->

    <owl:Class rdf:about="http://purl.org/tio/ns#Ticket">
        <rdfs:subClassOf rdf:resource="http://purl.org/goodrelations/v1#ProductOrService"/>
        <rdfs:comment xml:lang="en">A ticket is a tradeable right to access a particular event or location, or to use a particular transportation service.</rdfs:comment>
        <rdfs:isDefinedBy rdf:resource="http://purl.org/tio/ns#"/>
        <rdfs:label xml:lang="en">Ticket (gr:ProductOrService)</rdfs:label>
    </owl:Class>
    


    <!-- http://purl.org/tio/ns#TicketPlaceholder -->

    <owl:Class rdf:about="http://purl.org/tio/ns#TicketPlaceholder">
        <rdfs:subClassOf rdf:resource="http://purl.org/goodrelations/v1#ProductOrServicesSomeInstancesPlaceholder"/>
        <rdfs:subClassOf rdf:resource="http://purl.org/tio/ns#Ticket"/>
        <rdfs:comment xml:lang="en">A ticket placeholder is a dummy for multiple tickets that are themselves not exposed as data.</rdfs:comment>
        <rdfs:isDefinedBy rdf:resource="http://purl.org/tio/ns#"/>
        <rdfs:label xml:lang="en">TicketPlaceholder (gr:ProductOrService)</rdfs:label>
    </owl:Class>
    


    <!-- http://purl.org/tio/ns#TrainService -->

    <owl:Class rdf:about="http://purl.org/tio/ns#TrainService">
        <rdfs:subClassOf rdf:resource="http://purl.org/tio/ns#TransportationService"/>
        <rdfs:comment xml:lang="en">A regular or individual service to transport passengers or cargo from one location to another location by means of a train, subway, or other railroad vehicle

Note: By design, the Tickets Ontology does not provide mechanisms for modeling rules for recurring patterns of transportation services (e.g. every Monday at 8:00). Instead, it expects that you materialize each individual connection on a given day.
Most train schedule applications are complex databases, so they will have to be exposed as SPARQL endpoints anyway.</rdfs:comment>
        <rdfs:isDefinedBy rdf:resource="http://purl.org/tio/ns#"/>
        <rdfs:label xml:lang="en">TrainService</rdfs:label>
    </owl:Class>
    


    <!-- http://purl.org/tio/ns#TransportationService -->

    <owl:Class rdf:about="http://purl.org/tio/ns#TransportationService">
        <rdfs:subClassOf rdf:resource="http://purl.org/goodrelations/v1#ProductOrService"/>
        <rdfs:comment xml:lang="en">A service to transport passengers or cargo from one location to another location, with optionally intermediate stops

Note: By design, the Tickets Ontology does not provide mechanisms for modeling rules for recurring patterns of transportation services (e.g. every Monday at 8:00). Instead, it expects that you materialize each individual connection on a given day.
Most timetable applications are complex databases, so they will have to be exposed as SPARQL endpoints anyway.</rdfs:comment>
        <rdfs:isDefinedBy rdf:resource="http://purl.org/tio/ns#"/>
        <rdfs:label xml:lang="en">TransportationService</rdfs:label>
    </owl:Class>
    


    <!-- http://www.loa-cnr.it/ontologies/DUL.owl#Event -->

    <owl:Class rdf:about="http://www.loa-cnr.it/ontologies/DUL.owl#Event"/>
    


    <!-- 
    ///////////////////////////////////////////////////////////////////////////////////////
    //
    // Individuals
    //
    ///////////////////////////////////////////////////////////////////////////////////////
     -->

    


    <!-- http://purl.org/tio/ns#FirstClass -->

    <owl:NamedIndividual rdf:about="http://purl.org/tio/ns#FirstClass">
        <rdf:type rdf:resource="http://purl.org/tio/ns#ServiceLevel"/>
        <rdfs:comment xml:lang="en">First class as a service level / fare class for transportation by aircraft

Note: The exact character of a particular fare class may vary by carrier or country. 
You can create individual instances of tio:ServiceLevel for a particular fare class for a particular airline.</rdfs:comment>
        <rdfs:isDefinedBy rdf:resource="http://purl.org/tio/ns#"/>
        <rdfs:label xml:lang="en">FirstClass (tio:ServiceLevel)</rdfs:label>
    </owl:NamedIndividual>
</rdf:RDF>



<!-- Generated by the OWL API (version 4.5.9.2019-02-01T07:24:44Z) https://github.com/owlcs/owlapi -->

